Wrote bodies for priv_try_write_header, priv_try_encrypt_body, and priv_write_trailer in Session, along with some associated routines.

src/ByteBuf.dfy
@@ -1,26 +1,28 @@
 include "StandardLibrary.dfy"
 include "AwsCrypto.dfy"
+include "ByteOrder.dfy"
 
 module ByteBuffer {
   import opened StandardLibrary
   import opened Aws
+  import ByteOrder
+
+  // ---------- ByteBuf --------------------------------------------------
 
   // A ByteBuf is a slice of a byte array. Its capacity is the range buffer[start..end] and
   // its contents is buffer[start..start+len].
   datatype ByteBuf = ByteBuf(a: array<byte>, start: nat, end: nat, len: nat)
-  function ByteBufCapacity(bb: ByteBuf): int {
+  function method ByteBufCapacity(bb: ByteBuf): int {
     bb.end - bb.start
   }
   predicate GoodByteBuf(bb: ByteBuf) {
     bb.start <= bb.end <= bb.a.Length &&
     bb.len <= ByteBufCapacity(bb)
   }
-
-  // A ByteCursor represents a movable pointer within a byte array. It points to "len" bytes
-  // starting at position "start" in "a".
-  datatype ByteCursor = ByteCursor(a: array<byte>, start: nat, len: nat)
-  predicate GoodByteCursor(bc: ByteCursor) {
-    bc.start + bc.len <= bc.a.Length
+  function method ByteBufRemaining(bb: ByteBuf): nat
+    requires GoodByteBuf(bb)
+  {
+    ByteBufCapacity(bb) - bb.len
   }
 
   method ByteBufInit(capacity: nat) returns (bb: ByteBuf)
@@ -62,6 +64,20 @@ module ByteBuffer {
     ByteBuf(a, 0, capacity, 0)
   }
 
+  function method ByteBufAdvance(bb: ByteBuf, n: nat): ByteBuf
+    requires GoodByteBuf(bb) && n <= bb.len
+    ensures GoodByteBuf(ByteBufAdvance(bb, n))
+  {
+    ByteBuf(bb.a, bb.start + n, bb.end, bb.len - n)
+  }
+
+  function method ByteBufElongate(bb: ByteBuf, n: nat): ByteBuf
+    requires GoodByteBuf(bb) && n <= ByteBufRemaining(bb)
+    ensures GoodByteBuf(ByteBufElongate(bb, n))
+  {
+    bb.(len := bb.len + n)
+  }
+
   method ByteBufFill(bb: ByteBuf, b: byte)
     requires GoodByteBuf(bb)
     modifies bb.a
@@ -70,6 +86,15 @@ module ByteBuffer {
   {
     forall i | 0 <= i < bb.len {
       bb.a[bb.start + i] := b;
+    }
+  }
+
+  method ByteBufClear(bb: ByteBuf)
+    requires GoodByteBuf(bb)
+    modifies bb.a
+  {
+    forall i | bb.start <= i < bb.end {
+      bb.a[i] := 0;
     }
   }
 
@@ -93,6 +118,61 @@ module ByteBuffer {
     }
   }
 
+  /**
+   * Write specified number of bytes from array to byte buffer.
+   *
+   * On success, returns true and updates the buffer length accordingly.
+   * If there is insufficient space in the buffer, returns false, leaving the
+   * buffer unchanged.
+   */
+  method ByteBufWrite(buf: ByteBuf, src: array<byte>, len: nat) returns (success: bool, buf': ByteBuf)
+    requires GoodByteBuf(buf) && len <= src.Length
+    modifies buf.a
+    ensures GoodByteBuf(buf')
+    ensures !success ==> buf' == buf && forall i :: 0 <= i < buf.a.Length ==> buf.a[i] == old(buf.a[i])
+    ensures success ==> buf' == buf.(len := buf.len + len)
+  {
+    if ByteBufRemaining(buf) < len {
+      return false, buf;
+    }
+
+    forall i | 0 <= i < len {
+      buf.a[buf.start + buf.len + i] := src[i];
+    }
+    return true, buf.(len := buf.len + len);
+  }
+
+  /**
+   * Writes a 16-bit integer in network byte order (big endian) to buffer.
+   *
+   * On success, returns true and updates the cursor /length accordingly.
+   * If there is insufficient space in the cursor, returns false, leaving the
+   * cursor unchanged.
+   */
+  method ByteBufWriteBe16(bb: ByteBuf, x: nat) returns (success: bool, bb': ByteBuf)
+    requires GoodByteBuf(bb) && x < 0x1_0000
+    modifies bb.a
+    ensures bb' == if success then bb.(len := bb.len + 2) else bb
+  {
+    if ByteBufRemaining(bb) < 2 {
+      return false, bb;
+    }
+    var b1, b0 := ByteOrder.ToBytes2(x);
+    var n := bb.start + bb.len;
+    bb.a[n] := b1;
+    bb.a[n + 1] := b0;
+    return true, ByteBufElongate(bb, 2);
+  }
+
+  // ---------- ByteCursor --------------------------------------------------
+
+  // A ByteCursor represents a movable pointer within a byte array. It points to "len" bytes
+  // starting at position "start" in "a".
+  datatype ByteCursor = ByteCursor(a: array<byte>, start: nat, len: nat)
+  predicate GoodByteCursor(bc: ByteCursor) {
+    bc.start + bc.len <= bc.a.Length
+  }
+
   function method ByteCursorFromBuf(bb: ByteBuf): ByteCursor
     requires GoodByteBuf(bb)
     ensures GoodByteCursor(ByteCursorFromBuf(bb))
@@ -107,16 +187,27 @@ module ByteBuffer {
     ByteCursor(a, 0, len)
   }
 
-  function method ByteCursorAdvance(bc: ByteCursor, n: nat): (bool, ByteCursor)
+  method ByteCursorSplit(bc: ByteCursor, n: nat) returns (success: bool, bc0: ByteCursor, bc1: ByteCursor)  // aws_byte_cursor_advance
     requires GoodByteCursor(bc)
-    ensures var (success, bc') := ByteCursorAdvance(bc, n);
-      GoodByteCursor(bc')
+    ensures success ==> GoodByteCursor(bc0) && GoodByteCursor(bc1)
+    ensures !success ==> bc1 == bc
   {
-    var max := UINT64_MAX / 2;
-    if n <= max && n <= bc.len <= max then
-      var bc' := ByteCursor(bc.a, bc.start + n, bc.len - n);
-      (true, bc')
-    else
-      (false, bc)
+    if n <= bc.len {
+      bc0 := bc.(len := n);
+      bc1 := bc.(start := bc.start + n, len := bc.len - n);
+      success := true;
+    } else {
+      bc1 := bc;
+      success := false;
+    }
+  }
+
+  method ByteCursorClear(bc: ByteCursor)
+    requires GoodByteCursor(bc)
+    modifies bc.a
+  {
+    forall i | 0 <= i < bc.len {
+      bc.a[bc.start + i] := 0;
+    }
   }
 }
